working on infer pats

src/Typing.v
@@ -19,18 +19,14 @@ Require Import Arith.Arith_base.
 Require Import List.
 Require Import SimpleTypes.
 Require Import MyLtacs.
-
-(** * Non empty list for case expressions*)
-
-Inductive non_empty_list (A : Type) : Type :=
-  | one : A -> non_empty_list A
-  | cons' : A -> non_empty_list A -> non_empty_list A.
+Require Import NonEmptyList.
 
 (** * Pattern definition *)
 
 Inductive pat : Set :=
 | var_p : id -> pat
-| const_p : id -> pat.
+| const_p : id -> pat
+| list_p : (id * schm) -> list pat -> pat.
 
 (** * Lambda term definition *)
 
@@ -44,96 +40,106 @@ Inductive term : Set :=
 
 (** * Rules for typing patterns *)
 
-Inductive has_type_pat : ctx -> pat -> ty -> Prop:=
-| const_htp : forall x G, has_type_pat G (const_p x) (con x)
-| var_htp : forall x G sigma tau, in_ctx x G = Some sigma ->
-                             is_schm_instance tau sigma ->
-                             has_type_pat G (var_p x) tau.
-
-Inductive has_type_patterns : ctx -> non_empty_list pat -> ty -> Prop :=
-| one_pattern : forall G p tau, has_type_pat G p tau ->
-                           has_type_patterns G (one p) tau
-| many_pattern : forall G p ps tau, has_type_pat G p tau ->
-                               has_type_patterns G ps tau ->
-                               has_type_patterns G (cons' p ps) tau.
-
-(** * Syntax-directed rule system of Damas-Milner *)
-
-Fixpoint get_pats (c : non_empty_list (pat * term)) : non_empty_list pat :=
-  match c with
-  | one (p, _) => one p
-  | cons' (p, _) c' => cons' p (get_pats c')
+Definition not_arrow (tau : ty) : Prop :=
+  match tau with
+  | arrow _ _ => False
+  | _ => True
   end.
 
-Fixpoint get_terms (c : non_empty_list (pat * term)) : non_empty_list term :=
-  match c with
-  | one (_, t) => one t
-  | cons' (_, t) c' => cons' t (get_terms c')
+Definition not_arrow_dec (tau : ty) : bool :=
+  match tau with
+  | arrow _ _ => false
+  | _ => true
   end.
 
-Inductive has_type : ctx -> term -> ty -> Prop :=
-| const_ht : forall x G, has_type G (const_t x) (con x)
-| var_ht : forall x G sigma tau, in_ctx x G = Some sigma ->
-                            is_schm_instance tau sigma ->
-                            has_type G (var_t x) tau
-| lam_ht : forall x G tau tau' e, has_type ((x, ty_to_schm tau) :: G) e tau' ->
-                             has_type G (lam_t x e) (arrow tau tau')
-| app_ht : forall G tau tau' l rho, has_type G l (arrow tau tau') ->
-                               has_type G rho tau ->
-                               has_type G (app_t l rho) tau'
-| let_ht : forall G x e e' tau tau', has_type G e tau ->
-                                has_type ((x, gen_ty tau G) :: G) e' tau' ->
-                                has_type G (let_t x e e') tau'
-| case_ht : forall G e tau tau' cs, has_type G e tau ->
-                               has_type_patterns G (get_pats cs) tau ->
-                               has_type_terms G (get_terms cs) tau' ->
-                               has_type G (case_t e cs) tau'
-  with has_type_terms : ctx -> non_empty_list term -> ty -> Prop :=
-       | one_term : forall G e tau, has_type G e tau ->
-                                  has_type_terms G (one e) tau
-       | many_terms : forall G e tau es, has_type G e tau -> 
-                                         has_type_terms G es tau ->
-                                         has_type_terms G (cons' e es) tau.
+Fixpoint arguments_of_ty (tau : ty) : list ty :=
+  match tau with
+  | arrow tau1 tau2 => tau1::arguments_of_ty tau2
+  | _ => nil
+  end.
 
-Scheme has_type_mut := Induction for has_type Sort Prop
-with has_type_terms_mut := Induction for has_type_terms Sort Prop.
+Fixpoint return_of_ty (tau : ty) : ty :=
+  match tau with
+  | arrow tau1 tau2 => return_of_ty tau2
+  | tau' => tau'
+  end.
 
-(** * The Great Substitution Lemma *)
+Inductive has_type_pat : pat -> ty -> Prop:=
+| const_htp : forall x, has_type_pat (const_p x) (con x)
+| var_htp : forall x tau, has_type_pat (var_p x) tau
+| list_htp : forall x sigma ps tau, is_schm_instance tau sigma ->
+                               has_type_pats ps (arguments_of_ty tau) -> 
+                               has_type_pat (list_p (x, sigma) ps) (return_of_ty tau)
+with
+has_type_pats : list pat -> list ty -> Prop :=
+| no_pat : has_type_pats nil nil
+| many_pat : forall p ps tau taus, has_type_pat p tau ->
+                              has_type_pats ps taus  ->
+                              has_type_pats (p::ps) (tau::taus).
+
+Fixpoint get_pats (cs : non_empty_list (pat * term)) : non_empty_list pat :=
+  match cs with
+  | one (p, _) =>  one p
+  | cons' (p, _) cs' => cons' p (get_pats cs')
+  end.
+
+Fixpoint get_terms (cs : non_empty_list (pat * term)) : non_empty_list term :=
+  match cs with
+  | one (_, t) =>  one t
+  | cons' (_, t) cs' => cons' t (get_terms cs')
+  end.
+
+Scheme has_type_pat_mut := Minimality for has_type_pat Sort Prop
+with has_type_pats_mut := Minimality for has_type_pats Sort Prop.
 
 (** has_pat is stable under substitution *)
-Lemma has_type_pat_is_stable_under_substitution : forall e s G tau,
-    has_type_pat G e tau -> has_type_pat (apply_subst_ctx s G) e (apply_subst s tau).
+Lemma has_type_pat_is_stable_under_substitution : forall p s tau,
+    has_type_pat p tau -> has_type_pat p (apply_subst s tau).
 Proof.
-  induction e.
-  (** var case *)
-  - intros. inversion H.
-    subst.
-    econstructor.
-    + induction G; simpl in *; mysimp.
-      destruct a.
-      mysimp.
-      apply IHG.
-      econstructor.
-      apply H1.
-      assumption.
-      assumption.
-    + unfold is_schm_instance in *.
-      destruct H3.
-      eapply subst_inst_subst_type in H0.
-      exists (map_apply_subst_ty s x).
-      apply H0.
+  intros.
+  Admitted.
+  (*
+  apply (has_type_pat_mut
+           (fun (p'': pat) tau => forall s tau',
+                has_type_pat p'' tau' -> has_type_pat p'' (apply_subst s tau'))
+           (fun l (tau : ty) => forall s tau',
+                has_type_pats l tau' -> has_type_pats l (apply_subst s tau'))
+           ) with (p:=p) (t:=tau); intros; eauto.
   (** const case *)
-  - intros. inversion H.
-    subst.
+  - inverts* H0.
     econstructor.
+  (** var case *)
+  - econstructor; eauto.
+  (** list case *)
+  - inverts* H3.
+    apply list_htp with (tau1:=apply_subst s0 tau0).
+    rewrite <- apply_subst_arrow.
+    skip.
+    rewrite <- apply_subst_arrow.
+    eauto.
+  - inverts* H2.
+    econstructor.
+    fold (apply_subst s0 tau0).
+    eauto.
+  - inverts* H4.
+    econstructor.
+    + fold (apply_subst s0 tau0).
+      eauto.
+    + fold (apply_subst s0 tau4).
+      fold (apply_subst s0 tau5).
+      rewrite <- apply_subst_arrow.
+      eauto.
 Qed.
-
+*)
+      
 Hint Resolve has_type_pat_is_stable_under_substitution.
 
 (** has_patterns is stable under substitution *)
-Lemma has_type_patterns_is_stable_under_substitution : forall l s G tau,
-    has_type_patterns G l tau -> has_type_patterns (apply_subst_ctx s G) l (apply_subst s tau).
+(*
+Lemma has_type_patterns_is_stable_under_substitution : forall l s tau,
+    has_type_pats l tau -> has_type_pats l (apply_subst s tau).
 Proof.
+Admitted.
   induction l.
   - intros. inverts H.
     econstructor.
@@ -146,6 +152,41 @@ Proof.
 Qed.    
 
 Hint Resolve has_type_patterns_is_stable_under_substitution.
+*)
+
+(** * Syntax-directed rule system of Damas-Milner *)
+
+Inductive has_type : ctx -> term -> ty -> Prop :=
+| const_ht : forall x G, has_type G (const_t x) (con x)
+| var_ht : forall x G sigma tau, in_ctx x G = Some sigma ->
+                            is_schm_instance tau sigma ->
+                            has_type G (var_t x) tau
+| lam_ht : forall x G tau tau' e, has_type ((x, ty_to_schm tau) :: G) e tau' ->
+                             has_type G (lam_t x e) (arrow tau tau')
+| app_ht : forall G tau tau' l r, has_type G l (arrow tau tau') ->
+                               has_type G r tau ->
+                               has_type G (app_t l r) tau'
+| let_ht : forall G x e e' tau tau', has_type G e tau ->
+                                has_type ((x, gen_ty tau G) :: G) e' tau' ->
+                                has_type G (let_t x e e') tau'
+| case_ht : forall G e tau tau' cs, has_type G e tau ->
+                               has_type_cases G cs tau tau' ->
+                               has_type G (case_t e cs) tau'
+with
+has_type_cases : ctx -> non_empty_list (pat * term) -> ty -> ty -> Prop :=
+| one_term : forall G p e tau tau', has_type_pat p tau ->
+                                  has_type G e tau' -> 
+                                  has_type_cases G (one (p, e)) tau tau'
+| many_terms : forall G pe tau tau' cs, has_type_cases G (one pe) tau tau' -> 
+                                   has_type_cases G cs tau tau' ->
+                                   has_type_cases G (cons' pe cs) tau tau'.
+
+Scheme has_type_mut := Minimality for has_type Sort Prop
+with has_type_cases_mut := Minimality for has_type_cases Sort Prop.
+
+Check has_type_mut.
+
+(** * The Great Substitution Lemma *)
 
 (** has_type is stable under substitution *)
 Lemma has_type_is_stable_under_substitution : forall e s tau G,
@@ -153,16 +194,18 @@ Lemma has_type_is_stable_under_substitution : forall e s tau G,
 Proof.
   intros.
   apply (has_type_mut
-           (fun (G' : ctx) (e' : term) (tau' : ty) (h : has_type G' e' tau') => forall s tau G,
+           (fun (G' : ctx) (e' : term) (tau' : ty) => forall s tau G,
                          has_type G e' tau -> has_type (apply_subst_ctx s G) e' (apply_subst s tau))
-           (fun  (G' : ctx) (l' : non_empty_list term) (tau' : ty) (h : has_type_terms G' l' tau') => forall s tau G,
-              has_type_terms G l' tau -> has_type_terms (apply_subst_ctx s G) l' (apply_subst s tau))
+           (fun  (G' : ctx) (l' : non_empty_list (pat * term)) (tau' tau'' : ty) => forall s tau1 tau2 G,
+              has_type_cases G l' tau1 tau2 -> has_type_cases (apply_subst_ctx s G) l' (apply_subst s tau1) (apply_subst s tau2))
            ) with (c:=G) (t0:=tau); intros.
   (** const case *)
   - inverts* H0.
     econstructor.
   (** var case *)
-  - inversion H0.
+  - skip.
+    (*
+    inversion H2.
     subst.
     rename G into G', G1 into G.
     rename s into s', s0 into s.
@@ -182,15 +225,18 @@ Proof.
       eapply subst_inst_subst_type in H1.
       exists (map_apply_subst_ty s x).
       apply H1.
+*)
   (** lambda case *)
-  - inverts* H1.
+  - inverts* H2.
     rewrite apply_subst_arrow.
     econstructor.
-    rewrite <- ty_to_subst_schm. rewrite apply_subst_ctx_eq.
-    apply H0.
-    assumption.
+    rewrite <- ty_to_subst_schm.
+    rewrite apply_subst_ctx_eq.
+    auto.
     (** app case *)
-  - rename l into e1, rho into e2.
+  - skip.
+    (*
+    rename l into e1, rho into e2.
     rename s into s1, s0 into s.
     rename H0 into IHe1, H1 into IHe2.
     inverts* H2.
@@ -202,8 +248,11 @@ Proof.
     assumption.
     apply IHe2.
     assumption.
+*)
     (** let case *)
-  - inverts* H2.
+  - skip.
+    (*
+    inverts* H2.
     rename e0 into e1, e' into e2.
     rename s into s', s0 into s.
     rename tau into tau'', tau1 into tau.
@@ -235,31 +284,23 @@ Proof.
     erewrite <- gen_ty_renaming.
     assumption.
     apply r.
+*)
   (** case case *)
   - induction cs.
-    + simpl in *.
-      destruct a.
-      simpl in *.
-      inverts* h1.
-      inverts* H2.
+    + inverts* H4.
       econstructor.
-      eapply H0.
-      apply H6.
+      eapply H1.
+      apply H8.
       auto.
-      auto.
-    + destruct a as [p t].
-      inverts* H2.
-      simpl in *.
+    + inverts* H4.
       econstructor.
-      apply H0 with (tau:=tau2); eauto.
-      auto.
+      eapply H1; eauto.
       auto.
     (** terms one case *)
-  - intros.
-    inverts* H1.
+  - inverts* H3.
     econstructor; eauto.
     (** terms many case *)
-  - inverts* H2.
+  - inverts* H4.
     econstructor; eauto.
   - auto.
   - auto.
@@ -272,17 +313,30 @@ Lemma has_type_var_ctx_diff : forall (i j : id) (G : ctx) (tau : ty) (sigma : sc
 Proof.
   intros.
   inversion_clear H0.
- econstructor; crush.
+  econstructor; crush.
 Qed.
 
 Hint Resolve has_type_var_ctx_diff.
 
+(*
+Lemma has_type_pat_cons_commm : forall G i j  sigma1 sigma2 tau,
+    i <> j ->
+    has_type_pat ((i, sigma1) :: (j, sigma2) :: G) (var_p i) tau ->
+    has_type_pat ((j, sigma2) :: (i, sigma1) :: G) (var_p i) tau.
+Proof.
+  intros.
+  inversion H0.
+  subst.
+  
+
 Lemma has_type_pat_var_ctx_diff : forall (i j : id) (G : ctx) (tau : ty) (sigma : schm),
-    i <> j -> has_type_pat G (var_p i) tau -> has_type_pat ((j, sigma) :: G) (var_p i) tau.
+    i <> j -> has_type_pat (var_p i) tau -> has_type_pat ((j, sigma) :: G) (var_p i) tau.
 Proof.
   intros.
   inversion_clear H0.
- econstructor; crush.
+  econstructor.
+  econstructor; crush.
 Qed.
 
 Hint Resolve has_type_pat_var_ctx_diff.
+*)
